proof/crefine/Retype_C.thy
@@ -20,6 +20,8 @@ declare word_neq_0_conv [simp del]
 instance cte_C :: oneMB_size
   by intro_classes simp
 
+context begin interpretation Arch . (*FIXME: arch_split*)
+
 lemma sint_eq_uintI:
   "uint (a::word32) < 2^ (word_bits - 1) \<Longrightarrow> sint a = uint a"
   apply (rule word_sint.Abs_inverse')
@@ -72,6 +74,8 @@ definition
 where
   "ptr_retyps_gen n p mk_array
     = (if mk_array then ptr_arr_retyps n p else ptr_retyps n p)"
+
+end
 
 context kernel_m
 begin
@@ -2019,7 +2023,7 @@ proof (intro impI allI)
           Int_atLeastAtMost atLeastatMost_empty_iff split_paired_Ex 
 
   (* obj specific *)
-  have mko: "makeObjectKO (Inr ArchTypes_H.object_type.PageTableObject) = Some ko" by (simp add: ko_def makeObjectKO_def)
+  have mko: "makeObjectKO (Inr ARM_H.PageTableObject) = Some ko" by (simp add: ko_def makeObjectKO_def)
 
   have relrl:
     "cpte_relation makeObject (from_bytes (replicate (size_of TYPE(pte_C)) 0))"
@@ -2187,7 +2191,7 @@ proof (intro impI allI)
     by (clarsimp simp:range_cover_def[where 'a=32, folded word_bits_def])+
 
   (* obj specific *)
-  have mko: "makeObjectKO (Inr ArchTypes_H.object_type.PageDirectoryObject) = Some ko" 
+  have mko: "makeObjectKO (Inr ARM_H.PageDirectoryObject) = Some ko" 
     by (simp add: ko_def makeObjectKO_def)
 
   note blah[simp del] =  atLeastAtMost_iff atLeastatMost_subset_iff atLeastLessThan_iff
@@ -2379,20 +2383,20 @@ definition
                                               | ArchTypes_H.apiobject_type.EndpointObject \<Rightarrow> scast seL4_EndpointObject
                                               | ArchTypes_H.apiobject_type.NotificationObject \<Rightarrow> scast seL4_NotificationObject
                                               | ArchTypes_H.apiobject_type.CapTableObject \<Rightarrow> scast seL4_CapTableObject)
-                            | ArchTypes_H.SmallPageObject \<Rightarrow> scast seL4_ARM_SmallPageObject
-                            | ArchTypes_H.LargePageObject \<Rightarrow> scast seL4_ARM_LargePageObject  
-                            | ArchTypes_H.SectionObject \<Rightarrow> scast seL4_ARM_SectionObject
-                            | ArchTypes_H.SuperSectionObject \<Rightarrow> scast seL4_ARM_SuperSectionObject
-                            | ArchTypes_H.PageTableObject \<Rightarrow> scast seL4_ARM_PageTableObject
-                            | ArchTypes_H.PageDirectoryObject \<Rightarrow> scast seL4_ARM_PageDirectoryObject"
+                            | ARM_H.SmallPageObject \<Rightarrow> scast seL4_ARM_SmallPageObject
+                            | ARM_H.LargePageObject \<Rightarrow> scast seL4_ARM_LargePageObject  
+                            | ARM_H.SectionObject \<Rightarrow> scast seL4_ARM_SectionObject
+                            | ARM_H.SuperSectionObject \<Rightarrow> scast seL4_ARM_SuperSectionObject
+                            | ARM_H.PageTableObject \<Rightarrow> scast seL4_ARM_PageTableObject
+                            | ARM_H.PageDirectoryObject \<Rightarrow> scast seL4_ARM_PageDirectoryObject"
 
 lemmas nAPIObjects_def = seL4_NonArchObjectTypeCount_def
 
 lemma nAPIOBjects_object_type_from_H:
   "(scast nAPIObjects <=s object_type_from_H tp) = (toAPIType tp = None)"
-  by (simp add: toAPIType_def ArchTypes_H.toAPIType_def nAPIObjects_def
+  by (simp add: toAPIType_def nAPIObjects_def
     object_type_from_H_def word_sle_def api_object_defs "StrictC'_object_defs"
-    split: ArchTypes_H.object_type.splits ArchTypes_H.apiobject_type.splits)
+    split: ARM_H.object_type.splits ArchTypes_H.apiobject_type.splits)
 
 definition
   object_type_to_H :: "word32 \<Rightarrow> object_type"
@@ -2403,12 +2407,12 @@ definition
        if (x = scast seL4_EndpointObject) then APIObjectType ArchTypes_H.apiobject_type.EndpointObject else (
         if (x = scast seL4_NotificationObject) then APIObjectType ArchTypes_H.apiobject_type.NotificationObject else (
          if (x = scast seL4_CapTableObject) then APIObjectType ArchTypes_H.apiobject_type.CapTableObject else (
-          if (x = scast seL4_ARM_SmallPageObject) then ArchTypes_H.SmallPageObject else (
-           if (x = scast seL4_ARM_LargePageObject) then ArchTypes_H.LargePageObject else (
-            if (x = scast seL4_ARM_SectionObject) then ArchTypes_H.SectionObject else (
-             if (x = scast seL4_ARM_SuperSectionObject) then ArchTypes_H.SuperSectionObject else (
-              if (x = scast seL4_ARM_PageTableObject) then ArchTypes_H.PageTableObject else (
-               if (x = scast seL4_ARM_PageDirectoryObject) then ArchTypes_H.PageDirectoryObject else
+          if (x = scast seL4_ARM_SmallPageObject) then ARM_H.SmallPageObject else (
+           if (x = scast seL4_ARM_LargePageObject) then ARM_H.LargePageObject else (
+            if (x = scast seL4_ARM_SectionObject) then ARM_H.SectionObject else (
+             if (x = scast seL4_ARM_SuperSectionObject) then ARM_H.SuperSectionObject else (
+              if (x = scast seL4_ARM_PageTableObject) then ARM_H.PageTableObject else (
+               if (x = scast seL4_ARM_PageDirectoryObject) then ARM_H.PageDirectoryObject else
                 undefined)))))))))))"
 
 lemmas Kernel_C_defs =
@@ -2703,13 +2707,13 @@ lemma object_type_from_H_toAPIType_simps:
   "(object_type_from_H tp = scast seL4_EndpointObject) = (toAPIType tp = Some ArchTypes_H.apiobject_type.EndpointObject)"
   "(object_type_from_H tp = scast seL4_NotificationObject) = (toAPIType tp = Some ArchTypes_H.apiobject_type.NotificationObject)"
   "(object_type_from_H tp = scast seL4_CapTableObject) = (toAPIType tp = Some ArchTypes_H.apiobject_type.CapTableObject)"
-  "(object_type_from_H tp = scast seL4_ARM_SmallPageObject) = (tp = ArchTypes_H.SmallPageObject)"
-  "(object_type_from_H tp = scast seL4_ARM_LargePageObject) = (tp = ArchTypes_H.LargePageObject)"
-  "(object_type_from_H tp = scast seL4_ARM_SectionObject) = (tp = ArchTypes_H.SectionObject)"
-  "(object_type_from_H tp = scast seL4_ARM_SuperSectionObject) = (tp = ArchTypes_H.SuperSectionObject)"
-  "(object_type_from_H tp = scast seL4_ARM_PageTableObject) = (tp = ArchTypes_H.PageTableObject)"
-  "(object_type_from_H tp = scast seL4_ARM_PageDirectoryObject) = (tp = ArchTypes_H.PageDirectoryObject)"
-  by (auto simp: toAPIType_def ArchTypes_H.toAPIType_def
+  "(object_type_from_H tp = scast seL4_ARM_SmallPageObject) = (tp = ARM_H.SmallPageObject)"
+  "(object_type_from_H tp = scast seL4_ARM_LargePageObject) = (tp = ARM_H.LargePageObject)"
+  "(object_type_from_H tp = scast seL4_ARM_SectionObject) = (tp = ARM_H.SectionObject)"
+  "(object_type_from_H tp = scast seL4_ARM_SuperSectionObject) = (tp = ARM_H.SuperSectionObject)"
+  "(object_type_from_H tp = scast seL4_ARM_PageTableObject) = (tp = ARM_H.PageTableObject)"
+  "(object_type_from_H tp = scast seL4_ARM_PageDirectoryObject) = (tp = ARM_H.PageDirectoryObject)"
+  by (auto simp: toAPIType_def
                  object_type_from_H_def "StrictC'_object_defs" api_object_defs
           split: object_type.splits ArchTypes_H.apiobject_type.splits)
 
@@ -3053,7 +3057,7 @@ lemma cnc_tcb_helper:
                 (heap_update ((Ptr &((Ptr &((Ptr &(p\<rightarrow>[''tcbArch_C'']) :: arch_tcb_C ptr)\<rightarrow>[''tcbContext_C''])
                      :: user_context_C ptr)\<rightarrow>[''registers_C''])) :: (word32[18]) ptr)
                   (Arrays.update (h_val (hrs_mem a) ((Ptr &((Ptr &((Ptr &(p\<rightarrow>[''tcbArch_C'']) :: arch_tcb_C ptr)\<rightarrow>[''tcbContext_C''])
-                       :: user_context_C ptr)\<rightarrow>[''registers_C''])) :: (word32[18]) ptr)) (unat CPSR) (0x150 :: word32)))
+                       :: user_context_C ptr)\<rightarrow>[''registers_C''])) :: (word32[18]) ptr)) (unat Kernel_C.CPSR) (0x150 :: word32)))
                    (hrs_htd_update (\<lambda>xa. ptr_retyps_gen 1 (Ptr (ctcb_ptr_to_tcb_ptr p) :: (cte_C[5]) ptr) False
                        (ptr_retyps_gen 1 p False xa)) a)))) x)
              \<in> rf_sr"
@@ -4118,7 +4122,7 @@ lemma copyGlobalMappings_ccorres:
    apply (rule ccorres_h_t_valid_armKSGlobalPD)
    apply csymbr
    apply (rule ccorres_Guard_Seq)+
-   apply (simp add: kernelBase_def Platform.kernelBase_def objBits_simps archObjSize_def
+   apply (simp add: kernelBase_def ARM.kernelBase_def objBits_simps archObjSize_def
                     whileAnno_def word_sle_def word_sless_def
                     Collect_True              del: Collect_const)
    apply (rule_tac xf'="\<lambda>_. ()" in ccorres_abstract)
@@ -4305,7 +4309,7 @@ lemma upt_enum_offset_trivial:
      apply (simp add:max_word_def word_bits_def)
      done
    qed
-
+find_theorems name:getObjectSize_def
 lemma getObjectSize_max_size:
   "\<lbrakk> newType =  APIObjectType apiobject_type.Untyped \<longrightarrow> x < 32;
          newType =  APIObjectType apiobject_type.CapTableObject \<longrightarrow> x < 28 \<rbrakk> \<Longrightarrow> getObjectSize newType x < word_bits"
@@ -4780,6 +4784,8 @@ lemma placeNewObject_pde:
 
 end
 
+context begin interpretation Arch . (*FIXME: arch_split*)
+
 definition "placeNewObject_with_memset regionBase us \<equiv> 
   (do x \<leftarrow> placeNewObject regionBase UserData us;
       doMachineOp (mapM_x (\<lambda>p::word32. storeWord p (0::word32))
@@ -4788,6 +4794,8 @@ definition "placeNewObject_with_memset regionBase us \<equiv>
 
 crunch gsMaxObjectSize[wp]: placeNewObject_with_memset, createObject "\<lambda>s. P (gsMaxObjectSize s)"
   (wp: crunch_wps simp: unless_def)
+
+end
 
 context kernel_m begin
 
@@ -4994,7 +5002,7 @@ lemma Arch_createObject_ccorres:
      (createObject_hs_preconds regionBase newType userSize) 
      (createObject_c_preconds regionBase newType userSize)
      []
-     (ArchRetypeDecls_H.createObject newType regionBase userSize)
+     (ARM_H.createObject newType regionBase userSize)
      (Call Arch_createObject_'proc)"
 proof -
   note if_cong[cong]
@@ -5012,7 +5020,7 @@ proof -
     apply (cut_tac t)
     apply (case_tac newType,
            simp_all add: toAPIType_def ArchTypes_H.toAPIType_def
-               ArchRetype_H.createObject_def createPageObject_def bind_assoc
+               ARM_H.createObject_def createPageObject_def bind_assoc
                ARMLargePageBits_def)
 
          -- "SmallPageObject"
@@ -5446,7 +5454,7 @@ lemma threadSet_domain_ccorres [corres]:
 lemma createObject_ccorres:
   notes APITypecapBits_simps[simp] =
           APIType_capBits_def[split_simps
-          ArchTypes_H.object_type.split apiobject_type.split]
+          ARM_H.split apiobject_type.split]
   shows
     "ccorres ccap_relation ret__struct_cap_C_'
      (createObject_hs_preconds regionBase newType userSize)
@@ -5753,7 +5761,7 @@ proof -
     apply (auto simp: createObject_c_preconds_def objBits_simps field_simps
                split: apiobject_type.splits)[1]
    apply (clarsimp simp: nAPIObjects_def object_type_from_H_def Kernel_C_defs
-                  split: ArchTypes_H.object_type.splits)
+                  split: ARM_H.splits)
   apply (clarsimp simp: createObject_c_preconds_def
                         createObject_hs_preconds_def)
   done
@@ -6643,7 +6651,7 @@ shows "\<lbrace>P\<rbrace>createObject ty ptr us \<lbrace>\<lambda>m s. capRange
          apply wpc
              apply wp
         apply (simp add:split untypedRange.simps objBits_simps capRange_def APIType_capBits_def | wp)+
-       apply (simp add:ArchRetype_H.createObject_def capRange_def createPageObject_def APIType_capBits_def
+       apply (simp add:ARM_H.createObject_def capRange_def createPageObject_def APIType_capBits_def
          acapClass.simps | wp)+
   done
 
@@ -6798,9 +6806,9 @@ lemma createObject_child:
     apply clarsimp+
     apply (rename_tac arch_capability v0 v1 f)
     apply (case_tac arch_capability)
-     apply (simp add:ArchRetype_H.capUntypedSize_def)+
+     apply (simp add:ARM_H.capUntypedSize_def)+
      apply (simp add: is_aligned_no_wrap' field_simps)
-    apply (simp add:ArchRetype_H.capUntypedSize_def)+
+    apply (simp add:ARM_H.capUntypedSize_def)+
     apply (simp add: is_aligned_no_wrap' field_simps)
   apply clarsimp+
   done
@@ -6916,7 +6924,7 @@ shows
   apply (rule createObject_untypedRange)
   apply (clarsimp | wp)+
   apply (clarsimp simp: blah toAPIType_def APIType_capBits_def
-    ArchTypes_H.toAPIType_def split:ArchTypes_H.object_type.splits)
+    ArchTypes_H.toAPIType_def split:ARM_H.splits)
   apply (clarsimp simp:shiftl_t2n field_simps)
   apply (drule word_eq_zeroI)
   apply (drule(1) range_cover_no_0[where p = "Suc n"])
@@ -7120,7 +7128,7 @@ lemma APIType_capBits_min:
 end
 
 crunch gsCNodes[wp]: insertNewCap, Arch_createNewCaps, threadSet,
-        "ArchRetypeDecls_H.createObject" "\<lambda>s. P (gsCNodes s)"
+        "ARM_H.createObject" "\<lambda>s. P (gsCNodes s)"
   (wp: crunch_wps setObject_ksPSpace_only
      simp: unless_def updateObject_default_def ignore: getObject setObject)
 
