proof/crefine/TcbAcc_C.thy
@@ -212,7 +212,7 @@ lemma sanitiseRegister_spec:
                 Call sanitiseRegister_'proc
                 \<lbrace>\<acute>ret__unsigned_long = sanitiseRegister r v\<rbrace>"
   apply vcg
-  apply (auto simp: C_register_defs State_H.sanitiseRegister_def
+  apply (auto simp: C_register_defs ARM_H.sanitiseRegister_def
                     MachineTypes.sanitiseRegister_def word_0_sle_from_less
                  split: register.split)
   done
